src/impl/TLS13.Impl.ConnectionState.Repr.fsti
@@ -405,6 +405,11 @@ type certificate_verify_signature_snapshot = {
   cv_signature_len: SZ.t;
 }
 
+type certificate_chain_snapshot = {
+  certificate_chain_bytes_len: SZ.t;
+  certificate_chain_cert_count: SZ.t;
+}
+
 type key_schedule_snapshot = {
   snapshot_shared_secret_present: bool;
   snapshot_handshake_secret_present: bool;
